Primitives.dfy
@@ -3,15 +3,21 @@ module Primitives {
     import opened Std.Wrappers
     import C = Circuit
 
-    function behav_xor(inputs: map<C.CPort, bool>): Option<map<C.CPort, bool>>
+    function XorBehav(m: map<C.CPort, bool>): Option<map<C.CPort, bool>>
     {
-        if 0 !in inputs then
-            None
-        else if 1 !in inputs then
-            None
-        else
-            var o := if inputs[0] == inputs[1] then false else true;
+        if (0 in m) && (1 in m) then
+            var o := if m[0] == m[1] then false else true;
             Some(map[2 := o])
+        else
+            None
+    }
+
+    function AndBehav(m: map<C.CPort, bool>): Option<map<C.CPort, bool> >
+    {
+        if (0 in m) && (1 in m) then
+            Some(map[0 := m[0] && m[1]])
+        else
+            None
     }
 
     const nk_xor := C.CComb(
@@ -23,8 +29,8 @@ module Primitives {
             case (2, 1) => true
             case _ => false
         ),
-        Behav := behav_xor,
-        PortNames := C.PortNames2to1
+        Behav := XorBehav,
+        PortNames := PortNames2to1
     )
 
     const xor_port_bound: C.CPort := 3
@@ -34,8 +40,26 @@ module Primitives {
     {
     }
 
+    predicate BinaryPathExists(p: C.CPort, q: C.CPort)
+    {
+        (p in {0, 1}) && (q == 0)
+    }
 
-    //lemma XorValid()
-    //    ensures C.CNodeKindValid(
+    function PortNames2to1(name: string): Option<C.CPort>
+    {
+        match name
+        case "i0" => Some(0 as C.CPort)
+        case "i1" => Some(1 as C.CPort)
+        case "o" => Some(2 as C.CPort)
+        case _ => None
+    }
+
+    const nk_and: C.CNodeKind := C.CComb(
+        IPorts := {0 as C.CPort, 1 as C.CPort},
+        OPorts := {2 as C.CPort},
+        PathExists := BinaryPathExists,
+        Behav := AndBehav,
+        PortNames := PortNames2to1
+    )
 
 }
